

Cyclic derivatives and functions

Fire Fox

November 2025

Abstract

This paper presents an independent exploration of cyclic derivatives based on the fractional and complex-order derivatives paper made by the same Author.

Note to Readers: This represents independent rediscovery of classical fractional calculus concepts. I (The Author) present this work as a pedagogical exercise in mathematical exploration rather than novel research.

Background

The Main formula that works for all derivatives and can be used in the Maclaurin series

$$D^\alpha x^n = \frac{\Gamma(n+1)}{\Gamma(n-\alpha+1)} x^{n-\alpha}$$

The more important formulas that are built on this one

$$D^\alpha e^{ax} = a^\alpha e^{ax} \qquad e^{ix} = \cos(x) - i \sin(x)$$

$$e^x = \cosh(x) + \sinh(x) \qquad e^{-x} = \cosh(x) - \sinh(x)$$

$$D^\alpha \sin(x) = \sin\left(\frac{\alpha\pi}{2} + x\right) \qquad D^\alpha \cos(x) = \cos\left(\frac{\alpha\pi}{2} + x\right)$$

$$D^\alpha \sinh(x) = \frac{e^x - (-1)^\alpha e^{-x}}{2} \qquad D^\alpha \cosh(x) = \frac{e^x + (-1)^\alpha e^{-x}}{2}$$

1 Introduction

from what we have seen in the previous fractional and complex-order derivatives paper, cyclic derivatives are such a big area that deserves its own paper,

2 The foundation

From the fractional and complex-order derivatives paper, we know that

$$\text{when } a^n = 1, D^n(e^{ax}) = e^{ax} \text{ with } 2 \times n \text{ cyclic order}$$

And we can call that the theorem of cyclic derivatives

Theorem 1 *$f(x)$ is a cyclic derivative when $a^n = 1, D^n(e^{ax}) = e^{ax}$ with $2 \times n$ cyclic order*

And in the same paper, we generalized this to hold for any $k \equiv 0 \pmod{n}$

Theorem 2 *$f(x)$ is a lesser cyclic derivative when $a^n = 1, D^n(e^{ax}) = e^{ax}$ with $2 \times k$ cyclic order, where $k \equiv 0 \pmod{n}$*

With a hypothesis that I wish to prove in this paper, that

Hypothesis 1 *For every function cyclic derivatives that can be written in the form e^{ax} where $a^n = 1$ and satisfies the condition $2^n \in \mathbb{Z}^+$, there exists an algebraic perimetric form*

We can already see this for hyperbolic functions, where they can be written in the form $x^2 - y^2 = 1$, and trigonometric functions We also proved some equations

$$\begin{aligned} D^i e^{-x} &= e^{-(x+\pi)} = \cosh(x+\pi) - \sinh(x+\pi) \\ D^i \sinh(x) &= \frac{e^x - e^{-(x+\pi)}}{2} & D^i \cosh(x) &= \frac{e^x + e^{-(x+\pi)}}{2} \\ D^i e^{ix} &= e^{\frac{-\pi}{2}} \cos(x) + ie^{\frac{-\pi}{2}} \sin(x) \\ D^i \sin(x) &= \sin\left(\frac{i\pi}{2} + x\right) & D^i \cos(x) &= \cos\left(\frac{i\pi}{2} + x\right) \end{aligned}$$

and we also proved that for $\sin(x)$ and $\cos(x)$

3 More about the complex derivatives and known families

from what we know about $\sinh(x)$ and $\cosh(x)$ we can write their formulas in an other way

$$\begin{aligned} D^\alpha \sinh(x) &= \frac{e^x - (-1)^\alpha e^{-x}}{2} = \frac{e^x - (e^{i\pi})^\alpha e^{-x}}{2} = \frac{e^x - (e^{i\pi\alpha})e^{-x}}{2} \\ &= \frac{e^x - e^{i\pi\alpha-x}}{2} \end{aligned}$$

The same goes for $\cosh(x)$

$$D^\alpha \sinh(x) = \frac{e^x - e^{i\pi\alpha-x}}{2} \quad D^\alpha \cosh(x) = \frac{e^x + e^{i\pi\alpha-x}}{2}$$

We can see that we can't express them as simple forms, since the real value changes differently from the complex value. If we try to apply the derivative operator to e^x with the definition of $1 = e^{2i\pi}$, we get

$$D^\alpha e^x = 1^\alpha e^x = e^{2i0\alpha} e^x = e^x$$

We used that because it's the principal value

For trigonometric functions, we know that D^i represents a half turn before it changes to its integral from the real plane, but there is something to clarify

$$\text{Im}(D^i e^{ix}) = e^{\frac{-\pi}{2}} \sin(x)$$

As we can see, the first i -th derivative acts as a scaler that scales $\sin(x)$ by real value $e^{-\frac{\pi}{2}}$

However, this isn't equal to the $D^i \sin(x)$ as the definition changes from scaling to rotating, like this

$$D^i \sin(x) = \sin\left(\frac{i\pi}{2} + x\right) =$$

But since we have proven the multiplication law works in the framework, we can make sure that both are somewhat equal

$${}^i D^i e^{ix} = i^{i \times i} e^{ix} = (e^{\frac{i\pi}{2}})^{-1} e^{ix} = e^{\frac{-i\pi}{2}} e^{ix} = e^{ix - \frac{i\pi}{2}}$$

$$e^{i(x - \frac{\pi}{2})} = \cos\left(x - \frac{\pi}{2}\right) + i \sin\left(x - \frac{\pi}{2}\right) = \sin(x) - i \cos(x) = D^{-1} e^{ix} = \int e^{ix}$$

and for the sin we proved in the "Complex-order and fractional derivatives: first exploration" paper that the index law works on it, and thus the multiplication law either from here or from the series expansion, so that we can say

$${}^i D^i \sin(x) = \sin\left(\frac{i \times i\pi}{2} + x\right) = \sin\left(\frac{-\pi}{2} + x\right) = -\cos(x)$$

Thus, both of them work fine, just different prescriptive

We shall call the e^{ix} the complex perspective since it's all about the imaginary unit, and $\sin(x)$ the real perspective, even if there is i in it

3.1 The complex prescriptive

since D^i represents a whole rotation on the $D(i)$ plane, we can get more angles that could help us understand more what happens to the function to "integrate it"

first step is we are going to transform from i to $e^{\frac{i\pi}{2}}$ so we can deal with rotation with radians in circles

$$\begin{aligned} D^i e^{ax} &= D^{e^{\frac{i\pi}{2}}} e^{ax} & D^{-1} e^{ax} &= D^{e^{i\pi}} e^{ax} \\ D^{e^{i\theta}} e^{ax} &= a^{e^{i\theta}} e^{ax} & D^{e^{i\theta}} e^{ix} &= i^{e^{i\theta}} e^{ix} = e^{\frac{i\pi e^{i\theta}}{2}} e^{ix} = e^{i(\frac{\pi e^{i\theta}}{2} + x)} \end{aligned}$$

$$= \cos\left(\frac{\pi e^{i\theta}}{2} + x\right) + i \sin\left(\frac{\pi e^{i\theta}}{2} + x\right)$$

So now we can know what happens at the third of rotation or the third root of unity, which is equal to $\frac{\pi}{3}$ in radians, we get

$$D^{e^{\frac{i\pi}{3}}} e^{ix} = e^{i\left(\frac{\pi e^{\frac{i\pi}{3}}}{2} + x\right)} = \cos\left(\frac{\pi e^{\frac{i\pi}{3}}}{2} + x\right) + i \sin\left(\frac{\pi e^{\frac{i\pi}{3}}}{2} + x\right)$$

which after calculating $e^{\frac{i\pi}{3}}$ to be $\frac{1}{2} + i\frac{\sqrt{3}}{2}$ we can then multiply it by $\frac{\pi}{2}$ to get $\frac{\pi}{4} + i\frac{\pi\sqrt{3}}{4}$, then we plug it

$$e^{i\left(\frac{\pi}{4} + i\frac{\pi\sqrt{3}}{4} + x\right)} = e^{i\frac{\pi}{4} + i^2\frac{\pi\sqrt{3}}{4} + ix} = e^{i\left(x + \frac{\pi}{4}\right)} e^{-\frac{\pi\sqrt{3}}{4}} = e^{-\frac{\pi\sqrt{3}}{4}} \cos\left(x + \frac{\pi}{4}\right) + i e^{-\frac{\pi\sqrt{3}}{4}} \sin\left(x + \frac{\pi}{4}\right)$$

We can see that it scales by a factor of $e^{-\frac{\pi\sqrt{3}}{4}}$ and rotate with a factor of $\frac{\pi}{4}$
let's do the same for two-thirds, the value for $e^{\frac{2i\pi}{3}}$ to be $-\frac{1}{2} + i\frac{\sqrt{3}}{2}$ we can then multiply it again by $\frac{\pi}{2}$ to get $-\frac{\pi}{4} + i\frac{\pi\sqrt{3}}{4}$
Plugging it again, we get

$$e^{i\left(-\frac{\pi}{4} + i\frac{\pi\sqrt{3}}{4} + x\right)} = e^{-i\frac{\pi}{4} + i^2\frac{\pi\sqrt{3}}{4} + ix} = e^{i\left(x - \frac{\pi}{4}\right)} e^{-\frac{\pi\sqrt{3}}{4}} = e^{-\frac{\pi\sqrt{3}}{4}} \cos\left(x - \frac{\pi}{4}\right) + i e^{-\frac{\pi\sqrt{3}}{4}} \sin\left(x - \frac{\pi}{4}\right)$$

At two-thirds, it rotates with the same value but rotates backwards

Now we have a little information about what happens in the process of integrating such functions

at the first third of the way, it rotates by $\frac{\pi}{4}$ and scales by $e^{-\frac{\pi\sqrt{3}}{4}}$

For Halfway, it doesn't rotate but scales with a factor of $e^{-\frac{\pi}{2}}$

for two-thirds it rotates by $\frac{\pi}{4}$ and scales by $e^{-\frac{\pi\sqrt{3}}{4}}$

This may seem weird at the beginning until we notice that we aren't starting from order 1 or D^1 , we are starting from the zero point D^0 or the function itself, so the one-third and two-thirds don't cancel out on rotation, but they rotate to two different directions

The one-third rotates to D^1 and the two-thirds rotate to D^{-1} , while the middle point D^i doesn't rotate but scales because it's not a real derivative or real integral

We can even notice that in the first third we have $\cos\left(x + \frac{\pi}{4}\right)$ and $\sin\left(x + \frac{\pi}{4}\right)$, which are both pure half derivatives

$$D^{\frac{1}{2}} \sin(x) = \sin\left(\frac{\frac{1}{2}\pi}{2} + x\right) = \sin\left(\frac{\pi}{4} + x\right) \quad D^{\frac{1}{2}} \cos(x) = \cos\left(\frac{\frac{1}{2}\pi}{2} + x\right) = \cos\left(\frac{\pi}{4} + x\right)$$

and the same happens for the half-integer being rotated by $\frac{\pi}{4}$

3.2 The Real prescriptive

4 exploration into another cyclic derivatives

4.1 the third order cyclic derivatives

From the theorem, we can find the third cyclic derivative to be from the equation $a^3 = 1$, the solutions are going to be denoted by $1, \omega = \frac{1}{2} + i\frac{\sqrt{3}}{2}, \omega^2 = -\frac{1}{2} - i\frac{\sqrt{3}}{2}$ since one will result in e^x and is fully expected to be here because of Theorem 2, we are going to use ω

$$D^1 e^{\omega x} = \omega e^{\omega x} \quad D^2 e^{\omega x} = \omega^2 e^{\omega x} \quad D^3 e^{\omega x} = e^{\omega x}$$

We can call this function the third-order cyclic derivative, which comes between hyperbolic and trigonometric functions we will name them \sinh_3, \cosh_3 and $\sinh_3 \text{II}$ We can define them like this

$$D^\alpha \sinh_3(x) = \sinh_3 \text{II}(x) \quad \alpha \equiv 0 \pmod{3} \quad D^\alpha \sinh_3 \text{II}(x) = \cosh_3(x) \quad \alpha \equiv 1 \pmod{3}$$

$$D^\alpha \cosh_3(x) = \sinh_3(x) \quad \alpha \equiv 2 \pmod{3}$$

But this isn't the only way to define them, we can also define them with a series First we find the Maclaurin series for $e^{\omega x}$

$$e^{\omega x} = e^0 + \omega e^0 x + \frac{\omega^2 e^0 x^2}{2!} + \frac{e^0 x^3}{3!} + \dots = 1 + \omega x + \frac{\omega^2 x^2}{2!} + \frac{x^3}{3!} + \dots = \sum_{n=0}^{\infty} \frac{\omega^n x^n}{n!}$$

From this, we can divide them into three sums

$$\begin{aligned} & (1 + \frac{x^3}{3!} + \frac{x^6}{6!} + \dots) + \omega(x + \frac{x^4}{4!} + \frac{x^7}{7!} + \dots) + \omega^2(x^2 + \frac{x^5}{5!} + \frac{x^8}{8!} + \dots) \\ &= \sum_{n=0}^{\infty} \frac{x^{3n}}{(3n)!} + \omega \sum_{n=0}^{\infty} \frac{x^{3n+1}}{(3n+1)!} + \omega^2 \sum_{n=0}^{\infty} \frac{x^{3n+2}}{(3n+2)!} \end{aligned}$$

We can see that the first sum can be differentiated 3 times before going back to the first state, which is also for all the other sums, but since \sin and \sinh all have x^{an+1} , we are going to make the first function to be the second sum, to keep the naming consistent nothing more

So now we can define them to be

$$\sinh_3(x) = \sum_{n=0}^{\infty} \frac{x^{3n+1}}{(3n+1)!} \quad \sinh_3 \text{II}(x) = \sum_{n=0}^{\infty} \frac{x^{3n+2}}{(3n+2)!} \quad \cosh_3 = \sum_{n=0}^{\infty} \frac{x^{3n}}{(3n)!}$$

We can now define an equation that looks and acts like the Euler equation

$$e^{\omega x} = \cosh_3(x) + \omega \sinh_3(x) + \omega^2 \sinh_3 \text{II}(x)$$

We can now try to find one for ω^2

$$e^{\omega^2 x} = \sum_{n=0}^{\infty} \frac{(\omega^2)^n x^n}{n!}$$

at $3n$ we get $\omega^{6n} = 1$ so it's $\cosh_3(x)$, at $3n+1$ we get $\omega^{6n+2} = \omega^2$ so it's $\sinh_3(x)$ and at $3n$ we get $\omega^{6n+4} = \omega$ so it's $\sinh_3 \text{II}(x)$

$$e^{\omega^2 x} = \sum_{n=0}^{\infty} \frac{x^{3n}}{(3n)!} + \omega^2 \sum_{n=0}^{\infty} \frac{x^{3n+1}}{(3n+1)!} + \omega \sum_{n=0}^{\infty} \frac{x^{3n+2}}{(3n+2)!}$$

$$e^{\omega^2 x} = \cosh_3(x) + \omega^2 \sinh_3(x) + \omega \sinh_3 \text{II}(x)$$

and for e^x it's quite simple

$$e^x = 1 + x + \frac{x^2}{2!} + \frac{x^3}{3!} + \dots = \sum_{n=0}^{\infty} \frac{x^{3n}}{(3n)!} + \sum_{n=0}^{\infty} \frac{x^{3n+1}}{(3n+1)!} + \sum_{n=0}^{\infty} \frac{x^{3n+2}}{(3n+2)!}$$

$$e^x = \cosh_3(x) + \sinh_3(x) + \sinh_3 \text{II}(x)$$

like \sin and \sinh , we can try to find an exponent form for them

First, we begin by adding all of the equations so we have

$$e^x + e^{\omega x} + e^{\omega^2 x} = \cosh_3(x) + \sinh_3(x) + \sinh_3 \text{II}(x)$$

$$+ \cosh_3(x) + \omega \sinh_3(x) + \omega^2 \sinh_3 \text{II}(x) + \cosh_3(x) + \omega^2 \sinh_3(x) + \omega \sinh_3 \text{II}(x)$$

$$= 3 \cosh_3(x) + \sinh_3(x)(1 + \omega + \omega^2) + \sinh_3 \text{II}(x)(1 + \omega^2 + \omega)$$

and since we know that $1 + \omega + \omega^2 = 0$

$$e^x + e^{\omega x} + e^{\omega^2 x} = 3 \cosh_3(x) \quad \cosh_3(x) = \frac{e^x + e^{\omega x} + e^{\omega^2 x}}{3}$$

Now we can define the others by differentiating

$$\sinh_3(x) = \frac{e^x + \omega e^{\omega x} + \omega^2 e^{\omega^2 x}}{3} \quad \sinh_3 \text{II}(x) = \frac{e^x + \omega^2 e^{\omega x} + \omega e^{\omega^2 x}}{3}$$

since these definitions are going to continue with us, we shall call the $e^{ax} = \dots$ the **Euler form** and $f(x) = e^x + e^{ax} \dots$ the **exponentiation form**

4.2 Cyclic derivatives and Mittag-Leffler connection

4.3 Cyclic derivatives and prime numbers

4.4 Odd And Even cyclic derivatives

4.5 Cyclic derivatives and algebraic equations